src/cddl/pulse/CDDL.Pulse.Serialize.Gen.MapGroup.ZeroOrMore.Aux2.Lemma13.fsti
@@ -33,6 +33,7 @@ val invariant_insert_dup
   (gv: tvalue)
   (min_old: nat)
   (max_old: option nat)
+  (l: cbor_map)
 : Lemma
   (requires
     em == false /\
@@ -43,7 +44,7 @@ val invariant_insert_dup
     impl_serialize_map_zero_or_more_iterator_gen_invariant_min p sp1 sp2 except min v0 v /\
     impl_serialize_map_zero_or_more_iterator_gen_invariant_max p sp1 sp2 except max v0 v /\
     (exists (keq: EqTest.eq_test tkey) .
-      impl_serialize_map_zero_or_more_iterator_gen_invariant p sp1 sp2 except em out vout_old size count m v0 (map_of_list_cons keq gk gv v) min_old max_old true /\
+      impl_serialize_map_zero_or_more_iterator_gen_invariant p sp1 sp2 except em out vout_old size count m v0 (map_of_list_cons keq gk gv v) min_old max_old true l /\
       min == impl_serialize_map_zero_or_more_iterator_gen_update_min minl sp1 sp2 except min_old gk gv /\
       max == impl_serialize_map_zero_or_more_iterator_gen_update_max maxl sp1 sp2 except max_old gk gv /\
       sp1.serializable gk /\ sp2.serializable gv /\
@@ -51,5 +52,5 @@ val invariant_insert_dup
       cbor_map_defined (sp1.serializer gk) m)
   )
   (ensures
-    impl_serialize_map_zero_or_more_iterator_gen_invariant p sp1 sp2 except em out vout size count m v0 v min max false
+    impl_serialize_map_zero_or_more_iterator_gen_invariant p sp1 sp2 except em out vout size count m v0 v min max false l
   )
