src/cddl/pulse/CDDL.Pulse.Serialize.Gen.MapGroup.ZeroOrMore.Aux2.Proof0.fsti
@@ -38,7 +38,8 @@ val impl_serialize_map_zero_or_more_iterator_gen_invariant_implies_invariant1
   (min: nat)
   (max: option nat)
   (res: bool)
+  (l: cbor_map)
 : Lemma
-  (requires impl_serialize_map_zero_or_more_iterator_gen_invariant p sp1 sp2 except em out vout size count m v0 v min max res)
+  (requires impl_serialize_map_zero_or_more_iterator_gen_invariant p sp1 sp2 except em out vout size count m v0 v min max res l)
   (ensures impl_serialize_map_zero_or_more_iterator_gen_invariant1 p sp1 sp2 except em out vout size count m v0 v min max res)
-  [SMTPat (impl_serialize_map_zero_or_more_iterator_gen_invariant p sp1 sp2 except em out vout size count m v0 v min max res)]
+  [SMTPat (impl_serialize_map_zero_or_more_iterator_gen_invariant p sp1 sp2 except em out vout size count m v0 v min max res l)]
